feat: `match`-expressions with congruence equation theorems (#8506)
This PR implements `match`-expressions in `grind` using `match`
congruence equations. The goal is to minimize the number of `cast`
operations that need to be inserted, and avoid `cast` over functions.
The new approach support `match`-expressions of the form `match h : ...
with ...`.

src/Init/Grind/Util.lean
@@ -33,6 +33,55 @@ def offset (a b : Nat) : Nat := a + b
 def eqBwdPattern (a b : α) : Prop := a = b
 
 /--
+Gadget for representing generalization steps `h : x = val` in patterns
+This gadget is used to represent patterns in theorems that have been generalized to reduce the
+number of casts introduced during E-matching based instantiation.
+
+For example, consider the theorem
+```
+Option.pbind_some {α1 : Type u_1} {a : α1} {α2 : Type u_2}
+    {f : (a_1 : α1) → some a = some a_1 → Option α2}
+    : (some a).pbind f = f a rfl
+```
+Now, suppose we have a goal containing the term `c.pbind g` and the equivalence class
+`{c, some b}`. The E-matching module generates the instance
+```
+(some b).pbind (cast ⋯ g)
+```
+The `cast` is necessary because `g`'s type contains `c` instead of `some b.
+This `cast` problematic because we don't have a systematic way of pushing casts over functions
+to its arguments. Moreover, heterogeneous equality is not effective because the following theorem
+is not provable in DTT:
+```
+theorem hcongr (h₁ : f ≍ g) (h₂ : a ≍ b)  : f a ≍ g b := ...
+```
+The standard solution is to generalize the theorem above and write it as
+```
+theorem Option.pbind_some'
+        {α1 : Type u_1} {a : α1} {α2 : Type u_2}
+        {x : Option α1}
+        {f : (a_1 : α1) → x = some a_1 → Option α2}
+        (h : x = some a)
+        : x.pbind f = f a h := by
+  subst h
+  apply Option.pbind_some
+```
+Internally, we use this gadget to mark the E-matching pattern as
+```
+(genPattern h x (some a)).pbind f
+```
+This pattern is matched in the same way we match `(some a).pbind f`, but it saves the proof
+for the actual term to the `some`-application in `f`, and the actual term in `x`.
+
+In the example above, `c.pbind g` also matches the pattern `(genPattern h x (some a)).pbind f`,
+and stores `c` in `x`, `b` in `a`, and the proof that `c = some b` in `h`.
+-/
+def genPattern {α : Sort u} (_h : Prop) (x : α) (_val : α) : α := x
+
+/-- Similar to `genPattern` but for the heterogenous case -/
+def genHEqPattern {α β : Sort u} (_h : Prop) (x : α) (_val : β) : α := x
+
+/--
 Gadget for annotating the equalities in `match`-equations conclusions.
 `_origin` is the term used to instantiate the `match`-equation using E-matching.
 When `EqMatch a b origin` is `True`, we mark `origin` as a resolved case-split.
